coq.yalla/log_phase_sem.v
@@ -1,0 +1,526 @@
+(**************************************************************)
+(*   Copyright Dominique Larchey-Wendling [*]                 *)
+(*                                                            *)
+(*                             [*] Affiliation LORIA -- CNRS  *)
+(**************************************************************)
+(*      This file is distributed under the terms of the       *)
+(*         CeCILL v2 FREE SOFTWARE LICENSE AGREEMENT          *)
+(**************************************************************)
+
+(*   Adapted by Olivier Laurent [**]                          *)
+(*                                                            *)
+(*                              [**] Affiliation LIP -- CNRS  *)
+
+
+Require Import List_more List_Type Permutation_Type genperm_Type.
+
+Require Export closure_operators.
+
+Require Import ill_def.
+
+Import SetNotations.
+
+Notation " x '~[' b ']' y " := (PEperm_Type b x y) (at level 70, format "x  ~[ b ]  y").
+
+Notation "£" := ivar.
+Notation "⟙" := (itop).
+Notation "0" := (izero).
+Notation 𝝐 := (ione).
+Infix "﹠" := (iwith) (at level 50).
+Infix "⊗" := (itens) (at level 50).
+Infix "⊕" := (iplus) (at level 50).
+Infix "-o" := (ilmap) (at level 51, right associativity).
+Notation "x o- y" := (ilpam y x) (at level 52, left associativity).
+Notation "! x" := (ioc x) (at level 53).
+
+
+
+
+Set Implicit Arguments.
+
+Section PhaseSpaces.
+
+  Class MPhaseSpace (b : bool) := {
+    Web : Type;
+    PScompose : Web -> Web -> Web;
+    PSunit : Web;
+    PS_associative : m_associativity PScompose;
+    PS_neutral_l : m_neutrality_l PScompose PSunit;
+    PS_neutral_r : m_neutrality_r PScompose PSunit;
+    PSCL : @ClosureOp _ (@subset Web);
+    PScl_stable_l : @cl_stability_l _ _ PSCL (composes PScompose);
+    PScl_stable_r : @cl_stability_r _ _ PSCL (composes PScompose);
+    PSExp : Web -> Type;
+    PSsub_monoid_1 : @pwr_str_sub_monoid_hyp_1 _ PSunit PSExp;
+    PSsub_monoid_2 : @sub_monoid_hyp_2 _ subset (composes PScompose) PSExp;
+    PSsub_J : @pwr_sub_J_hyp _ PSCL PScompose PSunit PSExp;
+    PSsub_monoid_distr : @sub_monoid_distr_hyp _ subset (composes PScompose) glb PSExp;
+    PScl_commute : b = true -> @cl_commutativity _ _ PSCL (composes PScompose) }.
+
+  Infix "∘" := (composes PScompose) (at level 50, no associativity).
+  Infix "⊸" := (magicwand_l PScompose) (at level 51, right associativity).
+  Infix "⟜" := (magicwand_r PScompose) (at level 52, left associativity).
+  Notation "♯ x" := (glb PSExp x) (at level 40, no associativity).
+  Notation "❗ " := (@bang _ _ PSCL glb PSExp) (at level 40, no associativity).
+
+
+  Section MonadicInterpretation.
+
+    Variable perm_bool : bool.
+    Variable PS : MPhaseSpace perm_bool.
+
+    Definition list_compose l := fold_right (composes PScompose) (sg PSunit) l.
+
+    Fact list_compose_nil : list_compose nil = sg PSunit.
+    Proof. auto. Qed.
+
+    Fact list_compose_cons f l : list_compose (f :: l) = f ∘ list_compose l.
+    Proof. auto. Qed.
+
+    Notation "l ⊧  x" := (list_compose l ⊆ x) (at level 70, no associativity).
+    Notation "□" := (@cl _ _ PSCL).
+
+    Hint Resolve (@subset_refl Web) (@subset_preorder Web).
+    Hint Resolve (@composes_monotone _ PScompose).
+    Hint Resolve (@cl_idempotent _ _ PSCL).
+    Hint Resolve (@PScl_stable_l _ PS) (@PScl_stable_r _ PS)
+                 (@PS_associative _ PS) (@PS_neutral_l _ PS) (@PS_neutral_r _ PS)
+                 (@PSsub_monoid_1 _ PS) (@PSsub_monoid_2 _ PS) (@PSsub_J _ PS).
+    Hint Resolve  magicwand_l_adj_l magicwand_l_adj_r magicwand_r_adj_l magicwand_r_adj_r.
+
+
+    Fact list_compose_app l1 l2 : list_compose (l1 ++ l2) ≃ list_compose l1 ∘ list_compose l2.
+    Proof.
+    induction l1 as [ | f l IHl ]; simpl; split.
+    - apply (m_pwr_neutrality_l (@PS_neutral_l _ PS)).
+    - apply (m_pwr_neutrality_l (@PS_neutral_l _ PS)).
+    - etransitivity; [ | apply (m_pwr_associativity (@PS_associative _ PS)) ].
+      destruct IHl; apply composes_monotone; auto.
+    - etransitivity; [ apply (m_pwr_associativity (@PS_associative _ PS)) | ].
+      destruct IHl; apply composes_monotone; auto.
+    Qed.
+
+    Fact list_compose_monot_app l1 l2 m1 m2 x :
+      m1 ⊧ list_compose m2 -> l1 ++ m2 ++ l2 ⊧ x -> l1 ++ m1 ++ l2 ⊧ x.
+    Proof.
+    intros Hi H.
+    etransitivity; [ | apply H ].
+    etransitivity; [ | apply list_compose_app ].
+    etransitivity; [ apply list_compose_app | ].
+    apply composes_monotone; auto.
+    etransitivity; [ | apply list_compose_app ].
+    etransitivity; [ apply list_compose_app | ].
+    apply composes_monotone; auto.
+    Qed.
+
+    Fact list_compose_monot_cons l1 x y l2 z :
+      x ⊆ y -> l1 ++ y :: l2 ⊧ z -> l1 ++ x :: l2 ⊧ z.
+    Proof.
+    change (y :: l2) with ((y :: nil) ++ l2).
+    change (x :: l2) with ((x :: nil) ++ l2).
+    intros Hi.
+    apply list_compose_monot_app; simpl.
+    apply composes_monotone; auto.
+    Qed.
+
+    Notation lcap := (@fold_right (Web -> Type) _ glb top).
+
+    Hint Resolve glb_in glb_out_l glb_out_r top_greatest
+                 (m_pwr_cl_neutrality_l_2 (@PS_neutral_l _ PS)) (m_pwr_cl_neutrality_r_2 (@PS_neutral_r _ PS)).
+
+    Fact list_compose_bang l : □ (list_compose (map (fun x => ❗(□x)) l)) ≃ ❗ (lcap (map □ l)).
+    Proof.
+    eapply lcompose_store; eauto.
+    - apply sub_monoid_hyp_1_str, str_sub_monoid_1, PSsub_monoid_1; auto.
+    - apply (@sub_J_1 _ _ PScompose PSunit), PSsub_J.
+    - apply (@sub_J_2 _ _ PScompose PSunit), PSsub_J.
+    Qed.
+
+    Lemma sem_monad_r l x : l ⊧  x -> l ⊧ □x.
+    Proof. intros H; etransitivity; [ apply H | apply cl_increase ]. Qed.
+
+    Lemma sem_monad_l l1 l2 x y : l1 ++ x :: l2 ⊧ □y -> l1 ++ □x :: l2 ⊧ □y.
+    Proof.
+    intros H.
+    apply cl_le in H; auto.
+    transitivity (list_compose l1  ∘ □ (list_compose (x :: l2))).
+    - etransitivity; [ apply list_compose_app | ].
+      apply composes_monotone; auto; simpl.
+      apply PScl_stable_l.
+    - etransitivity; [ | apply H ].
+    etransitivity; [ apply PScl_stable_r | ].
+    apply cl_monotone.
+    etransitivity; [ | apply list_compose_app ]; auto.
+    Qed.
+
+    Lemma sem_monad_list_l l1 l2 l x :
+      l1 ++ l ++ l2 ⊧ □x -> list_compose l1 ∘ (□(list_compose l) ∘ list_compose l2) ⊆ □x.
+    Proof.
+    intros H.
+    assert (list_compose l1 ∘ (list_compose l ∘ list_compose l2) ⊆ □ x) as H'.
+    { etransitivity; [ | apply H ].
+      etransitivity; [ | apply list_compose_app ].
+      apply composes_monotone; auto.
+      apply list_compose_app. }
+    apply cl_le in H'; auto.
+    etransitivity; [ | apply H' ].
+    etransitivity; [ | apply PScl_stable_r ].
+    apply composes_monotone; auto.
+    Qed.
+
+    Fact sem_ax x : x :: nil ⊧ x.
+    Proof. apply (m_pwr_neutrality_r (@PS_neutral_r _ PS)). Qed.
+
+    Fact sem_cut Γ ϴ Δ x y : Γ ⊧ x -> Δ ++ x :: ϴ ⊧ y -> Δ ++ Γ ++ ϴ ⊧ y.
+    Proof.
+    intros H1 H2.
+    change (x :: ϴ) with ((x :: nil) ++ ϴ) in H2.
+    apply list_compose_monot_app with (x :: nil); auto; simpl.
+    etransitivity; [ apply H1 | ]; auto.
+    apply (m_pwr_neutrality_r (@PS_neutral_r _ PS)).
+    Qed.
+
+    Fact sem_swap (HPerm: perm_bool = true) Γ Δ x y z : Γ ++ x :: y :: Δ ⊧ □z -> Γ ++ y :: x :: Δ ⊧ □z.
+    Proof.
+    intros H.
+    change (x::y::Δ) with ((x::y::nil)++Δ) in H.
+    change (y::x::Δ) with ((y::x::nil)++Δ).
+    apply sem_monad_list_l in H.
+    etransitivity; [ | apply H ].
+    etransitivity; [ apply list_compose_app | ].
+    apply composes_monotone; auto.
+    etransitivity; [ apply list_compose_app | ].
+    apply composes_monotone; auto; simpl.
+    etransitivity; [ apply (m_pwr_associativity (@PS_associative _ PS)) | ].
+    etransitivity; [ | apply cl_monotone, (m_pwr_associativity (@PS_associative _ PS)) ].
+    etransitivity; [ | apply PScl_stable_l ].
+    apply composes_monotone; auto.
+    apply PScl_commute; auto.
+    Qed.
+
+    Fact sem_perm Γ Δ x : perm_bool = true -> Permutation_Type Γ Δ -> Γ ⊧ □x -> Δ ⊧ □x.
+    Proof.
+    intros Hb HP; revert x; induction HP as [ | a Ga De H1 IH1 | | ] ; intros c; auto.
+      + intros H; simpl; apply magicwand_l_adj_r; auto.
+        etransitivity; [ | apply (@cl_magicwand_l_1 _ _ _ _ (composes PScompose)) ]; auto.
+        apply IH1.
+        etransitivity; [ | apply cl_increase ]; auto.
+      + apply sem_swap with (Γ := nil) ; assumption.
+    Qed.
+
+(* TODO Universe inconsistency in log_cut_elim: even just the statement creates inconsistency
+    Fact sem_perm_0 b Γ Δ x : perm_bool = b -> Γ ~[b] Δ -> Γ ⊧ □x -> Δ ⊧ □x.
+    Proof.
+    destruct b; intros Hbool HP; revert x.
+    - induction HP as [ | a Ga De H1 IH1 | | ] ; intros c; auto.
+      + intros H; simpl; apply magicwand_l_adj_r; auto.
+        etransitivity; [ | apply (@cl_magicwand_l_1 _ _ _ _ (composes PScompose)) ]; auto.
+        apply IH1.
+        etransitivity; [ | apply cl_increase ]; auto.
+      + apply sem_swap with (Γ := nil) ; assumption.
+    - simpl in HP; rewrite HP; tauto.
+    Qed.
+
+    Fact sem_perm Γ Δ x : Γ ~[perm_bool] Δ -> Γ ⊧ □x -> Δ ⊧ □x.
+    Proof. intros HP; apply sem_perm_0 with perm_bool; auto. Qed.
+*)
+
+    Fact sem_tens_l Γ Δ x y z : Γ ++ x :: y :: Δ ⊧ z -> Γ ++ x ∘ y :: Δ ⊧ z.
+    Proof.
+    change (x::y::Δ) with ((x::y::nil)++Δ).
+    change (x ∘ y :: Δ) with ((x ∘ y :: nil) ++ Δ).
+    intros H; apply list_compose_monot_app with (x :: y :: nil); simpl; auto.
+    apply (m_pwr_associativity (@PS_associative _ PS)).
+    Qed.
+
+    Fact sem_tens_r Γ Δ x y : Γ ⊧ x -> Δ ⊧ y -> Γ ++ Δ ⊧ x ∘ y.
+    Proof.
+    intros H1 H2.
+    etransitivity; [ apply list_compose_app | ].
+    apply composes_monotone; auto.
+    Qed.
+
+    Fact sem_one_l_0 Γ Δ x : Γ ++ Δ ⊧ x -> Γ ++ (sg PSunit :: nil) ++ Δ ⊧ x.
+    Proof.
+    intros H.
+    change Δ with (nil ++ Δ) in H.
+    apply list_compose_monot_app with nil; auto.
+    apply sem_ax.
+    Qed.
+
+    Fact sem_one_l Γ Δ x : Γ ++ Δ ⊧ x -> Γ ++ sg PSunit :: Δ ⊧ x.
+    Proof. intros H; apply sem_one_l_0; auto. Qed.
+
+    Fact sem_one_r : nil ⊧ sg PSunit.
+    Proof. reflexivity. Qed.
+
+    Fact sem_limp_l Γ ϴ Δ x y z : Γ ⊧ x -> ϴ ++ y :: Δ ⊧ z -> ϴ ++ Γ ++ x ⊸ y :: Δ ⊧ z.
+    Proof.
+    intros H1 H2.
+    change (y :: Δ) with ((y :: nil) ++ Δ) in H2.
+    replace (Γ ++ x ⊸ y :: Δ) with ((Γ ++ x ⊸ y :: nil) ++ Δ) by (list_simpl; reflexivity).
+    apply list_compose_monot_app with (y :: nil); auto.
+    etransitivity; [ apply list_compose_app | ].
+    apply magicwand_l_adj_r; auto.
+    etransitivity; [ apply sem_ax | ].
+    apply (@magicwand_l_monotone _ _ _ (composes PScompose)); auto.
+    apply (m_pwr_neutrality_r (@PS_neutral_r _ PS)).
+    Qed.
+
+    Fact sem_limp_r Γ x y : x :: Γ ⊧ y -> Γ ⊧ x ⊸ y.
+    Proof. auto. Qed.
+
+    Fact sem_rimp_l Γ ϴ Δ x y z : Γ ⊧ x -> ϴ ++ y :: Δ ⊧ z -> ϴ ++ y ⟜ x :: Γ ++ Δ ⊧ z.
+    Proof.
+    intros H1 H2.
+    change (y :: Δ) with ((y :: nil) ++ Δ) in H2.
+    replace (y ⟜ x :: Γ ++ Δ) with ((y ⟜ x :: Γ) ++ Δ) by (list_simpl; reflexivity).
+    apply list_compose_monot_app with (y :: nil); auto; simpl.
+    apply magicwand_r_adj_r; auto.
+    apply (@magicwand_r_monotone _ _ _ (composes PScompose)); auto.
+    apply (m_pwr_neutrality_r (@PS_neutral_r _ PS)).
+    Qed.
+
+    Fact sem_rimp_r Γ x y : Γ ++ x :: nil ⊧ y -> Γ ⊧ y ⟜ x.
+    Proof.
+    intros H.
+    apply magicwand_r_adj_l.
+    etransitivity; [ | apply H ].
+    etransitivity; [ | apply list_compose_app ].
+    apply composes_monotone; auto.
+    apply (m_pwr_neutrality_r (@PS_neutral_r _ PS)).
+    Qed.
+
+    Fact sem_with_l1 Γ Δ x y z : Γ ++ x :: Δ ⊧ z -> Γ ++ x ∩ y :: Δ ⊧ z.
+    Proof. intros H; apply list_compose_monot_cons with x; auto; intros ?; tauto. Qed.
+
+    Fact sem_with_l2 Γ Δ x y z : Γ ++ y :: Δ ⊧ z -> Γ ++ x ∩ y :: Δ ⊧ z.
+    Proof. intros H; apply list_compose_monot_cons with y; auto; intros ?; tauto. Qed.
+
+    Fact sem_with_r Γ x y : Γ ⊧ x -> Γ ⊧ y -> Γ ⊧ x ∩ y.
+    Proof. intros H1 H2; split; auto. Qed.
+
+    Fact sem_plus_l Γ Δ x y z : Γ ++ x :: Δ ⊧ z -> Γ ++ y :: Δ ⊧ z -> Γ ++ x ∪ y :: Δ ⊧ z.
+    Proof.
+    intros H1 H2.
+    etransitivity; [ apply list_compose_app | ].
+    apply magicwand_l_adj_r; auto; simpl.
+    apply magicwand_r_adj_r; auto.
+    assert (x ⊆ list_compose Γ ⊸ z ⟜ list_compose Δ) as H1'.
+    { apply magicwand_r_adj_l, magicwand_l_adj_l; auto; simpl.
+      rewrite <- list_compose_cons.
+      etransitivity; [ apply list_compose_app | ]; auto. }
+    assert (y ⊆ list_compose Γ ⊸ z ⟜ list_compose Δ) as H2'.
+    { apply magicwand_r_adj_l, magicwand_l_adj_l; auto; simpl.
+      rewrite <- list_compose_cons.
+      etransitivity; [ apply list_compose_app | ]; auto. }
+    intros a [Ha | Ha]; auto.
+    Qed.
+
+    Fact sem_plus_r1 Γ x y : Γ ⊧ x -> Γ ⊧ x ∪ y.
+    Proof. intros H; (etransitivity; [ apply H | ]); intros ?; auto. Qed.
+    Fact sem_plus_r2 Γ x y : Γ ⊧ y -> Γ ⊧ x ∪ y.
+    Proof. intros H; (etransitivity; [ apply H | ]); intros ?; auto. Qed.
+
+    Fact sem_top_r Γ : Γ ⊧ top.
+    Proof. apply top_greatest. Qed.
+
+    Fact sem_zero_l Γ Δ x : Γ ++ ∅ :: Δ ⊧ x.
+    Proof.
+    etransitivity; [ apply list_compose_app | ].
+    apply magicwand_l_adj_r; auto.
+    apply magicwand_r_adj_r; auto.
+    intros z HF; inversion HF.
+    Qed.
+
+(* TODO try to remove some □: in the rules or in the definition of ❗ *)
+    Fact sem_bang_l Γ Δ x y : Γ ++ □x :: Δ ⊧ y -> Γ ++ ❗(□x) :: Δ ⊧ y.
+    Proof.
+    intros H.
+    apply list_compose_monot_cons with (□x); auto.
+    apply store_dec; auto.
+    Qed.
+
+    Fact sem_weak Γ Δ x y : Γ ++ □(sg PSunit) :: Δ ⊧ y -> Γ ++ ❗x :: Δ ⊧ y.
+    Proof.
+    intros H.
+    apply list_compose_monot_cons with (□(sg PSunit)); auto.
+    apply store_inc_unit; auto.
+    apply (@sub_J_1 _ _ PScompose PSunit), PSsub_J.
+    Qed.
+
+    Fact sem_cntr Γ Δ x y : Γ ++ ❗x :: ❗x :: Δ ⊧ □y -> Γ ++ ❗x :: Δ ⊧ □y.
+    Proof.
+    intros H.
+    change (❗x::❗x::Δ) with ((❗x::❗x::nil)++Δ) in H.
+    change (❗x::Δ) with ((❗x::nil)++Δ).
+    apply sem_monad_list_l in H.
+    etransitivity; [ | apply H ].
+    etransitivity; [ apply list_compose_app | ].
+    apply composes_monotone; auto.
+    etransitivity; [ apply list_compose_app | ].
+    apply composes_monotone; auto; simpl.
+    transitivity (❗x); [ apply (m_pwr_neutrality_r (@PS_neutral_r _ PS)) | ].
+    etransitivity; [ |    apply cl_monotone, (m_pwr_associativity (@PS_associative _ PS)) ].
+    etransitivity ; [ | apply cl_monotone, (m_pwr_neutrality_r (@PS_neutral_r _ PS)) ].
+    eapply store_compose_idem; eauto.
+    apply (@sub_J_2 _ _ PScompose PSunit), PSsub_J.
+    Qed.
+
+    Fact sem_bang_r Γ x : map (fun z => ❗(□z)) Γ ⊧ □x -> map (fun z => ❗(□z)) Γ ⊧ ❗(□x).
+    Proof.
+    intros H.
+    apply le_cl; auto.
+    etransitivity; [ apply list_compose_bang | ].
+    etransitivity; [ | apply store_der ]; auto.
+    etransitivity; [ apply list_compose_bang | ].
+    apply cl_closed; auto.
+    Qed.
+
+    Fact sem_oc_swap Γ Δ x y z : Γ ++ ❗(□x) :: ❗(□y) :: Δ ⊧ □z -> Γ ++ ❗(□y) :: ❗(□x) :: Δ ⊧ □z.
+    Proof.
+    intros H.
+    change (❗(□x)::❗(□y)::Δ) with ((❗(□x)::❗(□y)::nil)++Δ) in H.
+    change (❗(□y)::❗(□x)::Δ) with ((❗(□y)::❗(□x)::nil)++Δ).
+    apply sem_monad_list_l in H.
+    etransitivity; [ | apply H ].
+    etransitivity; [ apply list_compose_app | ].
+    apply composes_monotone; auto.
+    etransitivity; [ apply list_compose_app | ].
+    apply composes_monotone; auto; simpl.
+    etransitivity; [ apply (m_pwr_associativity (@PS_associative _ PS)) | ].
+    etransitivity; [ | apply cl_monotone, (m_pwr_associativity (@PS_associative _ PS)) ].
+    etransitivity; [ | apply PScl_stable_l ].
+    apply composes_monotone; auto.
+    etransitivity; [ | apply (@store_comp_2 _ _ _ PSCL) ]; auto;
+      [ | apply (@sub_J_2 _ _ PScompose PSunit), PSsub_J ].
+    transitivity (❗(glb (□y) (□x))).
+    - etransitivity; [ | eapply (@store_comp _ _ _ PSCL (composes PScompose) _ _ _ (sg PSunit)) ]; auto.
+      + etransitivity; [ | apply cl_increase ]; auto.
+      + apply (@sub_J_1 _ _ PScompose PSunit), PSsub_J.
+      + apply (@sub_J_2 _ _ PScompose PSunit), PSsub_J.
+    - apply store_monotone; auto.
+    Unshelve. all: auto.
+    Qed.
+
+    Fact sem_oc_perm Γ Δ ϴ ϴ' x : Permutation_Type ϴ ϴ' ->
+      Γ ++ map (fun z => ❗(□z)) ϴ ++ Δ ⊧ □x -> Γ ++ map (fun z => ❗(□z)) ϴ' ++ Δ ⊧ □x.
+    Proof.
+    intros HP; revert Γ Δ; induction HP as [ | a Ga De H1 IH1 | | ] ; intros Γ Δ H; auto.
+    - simpl.
+      change ((❗) (□ a) :: map (fun z : Web -> Type => (❗) (□ z)) De ++ Δ)
+        with (((❗) (□ a) :: nil) ++ map (fun z : Web -> Type => (❗) (□ z)) De ++ Δ).
+      rewrite app_assoc.
+      apply IH1; list_simpl; auto.
+    - apply sem_oc_swap; auto.
+    Qed.
+
+  End MonadicInterpretation.
+
+
+  (* Interpretation of Linear Logic *)
+
+  Section FormulaInterpretation.
+
+    Variable perm_bool : bool.
+    Variable PS : MPhaseSpace perm_bool.
+    Variable v : IAtom -> Web -> Type.
+    Notation "□" := (@cl _ _ PSCL).
+
+    Reserved Notation "⟦ A ⟧" (at level 49).
+    Fixpoint form_presem f :=
+      match f with
+      | 0     => ∅
+      | ⟙             => top
+      | 𝝐              => sg PSunit
+      | £ x    => v x
+      | a -o b => ⟦a⟧ ⊸ □(⟦b⟧)
+      | ineg a => ⟦a⟧ ⊸ □(v atN)
+      | b o- a => □(⟦b⟧) ⟜ ⟦a⟧
+      | igen a => □(v atN) ⟜ ⟦a⟧
+      | a ⊗ b  => ⟦a⟧ ∘ ⟦b⟧
+      | a ⊕ b  => ⟦a⟧ ∪ ⟦b⟧
+      | a ﹠ b  => □(⟦a⟧) ∩ □(⟦b⟧)
+      | !a     => ❗(□(⟦a⟧))
+      end
+    where "⟦ a ⟧" := (form_presem a).
+
+    Definition list_form_presem l := list_compose PS (map form_presem l).
+
+  End FormulaInterpretation.
+
+  Class MPhaseModel (P : ipfrag) := {
+    PMPS : MPhaseSpace (ipperm P);
+    PMval : IAtom -> Web -> Type;
+    PMgax : forall a, list_form_presem PMPS PMval (fst (projT2 (ipgax P) a))
+                    ⊆ @cl _ _ PSCL (form_presem PMPS PMval (snd (projT2 (ipgax P) a))) }.
+
+  Context { P : ipfrag }.
+  Variable PM : MPhaseModel P.
+
+  Infix "∘" := (composes PScompose) (at level 50, no associativity).
+  Notation "l ⊧  x" := (@list_compose _ PMPS l ⊆ x) (at level 70, no associativity).
+  Notation "□" := (@cl _ _ PSCL).
+  Notation Int := (@form_presem _ PMPS PMval).
+  Notation "l ⊢ x" := (ill P l x) (at level 70, no associativity).
+
+  Hint Resolve  magicwand_l_adj_l magicwand_l_adj_r magicwand_r_adj_l magicwand_r_adj_r.
+  Hint Resolve (@sem_monad_l _ PMPS).
+  Hint Resolve (@sem_one_r _ PMPS) (@sem_one_l _ PMPS) (@sem_tens_r _ PMPS) (@sem_tens_l _ PMPS)
+               (@sem_rimp_r _ PMPS) (@sem_rimp_l _ PMPS) (@sem_limp_r _ PMPS) (@sem_limp_l _ PMPS)
+               (@sem_with_r _ PMPS) (@sem_with_l1 _ PMPS) (@sem_with_l2 _ PMPS)
+               (@sem_plus_l _ PMPS) (@sem_zero_l _ PMPS)
+               (@sem_bang_r _ PMPS) (@sem_bang_l _ PMPS) (@sem_weak _ PMPS) (@sem_cntr _ PMPS).
+
+  Lemma int_ioc_list l : map Int (map ioc l) = map (fun z => ❗(□z)) (map Int l).
+  Proof. induction l; auto; simpl; rewrite IHl; auto. Qed.
+
+  Theorem ill_soundness Γ a : Γ ⊢ a -> map Int Γ ⊧ □(Int a).
+  Proof.
+  intros pi; induction pi;
+    (try rewrite ? map_app);
+    (try rewrite ? map_app in IHpi); (try rewrite ? map_app in IHpi1); (try rewrite ? map_app in IHpi2);
+    (try rewrite int_ioc_list); (try rewrite int_ioc_list in IHpi);
+    (try now (apply (@sem_monad_r _ PMPS); simpl; auto));
+    (try now (simpl; auto)).
+  - apply (@sem_monad_r _ PMPS), sem_ax.
+  - assert ({ipperm P = true} + {ipperm P = false}) as Hbool
+      by (clear; destruct (ipperm P); [ left | right ]; reflexivity).
+    destruct Hbool as [Hbool | Hbool]; intros; rewrite Hbool in p.
+    + apply sem_perm with (map Int l1); auto.
+      apply Permutation_Type_map; assumption.
+    + rewrite <- p; auto.
+(* TODO cf Universe inconsistency in sem_perm_0
+ eapply (@sem_perm _ PMPS); try eassumption.
+    apply PEperm_Type_map; assumption.
+*)
+  - apply sem_oc_perm with (map Int lw); auto.
+    apply Permutation_Type_map; assumption.
+  - transitivity (□ (□(Int A) ∘ □(Int B))); auto.
+    + apply (@sem_monad_r _ PMPS); auto.
+(* TODO use rules *)
+    + apply cl_le; [ apply subset_preorder | ]; simpl.
+      apply cl_stable; [ apply subset_preorder | apply PScl_stable_l | apply PScl_stable_r ].
+  - simpl; apply list_compose_monot_cons with (□ (Int B) ⟜ □ (Int A)); auto.
+    + eapply (@magicwand_r_eq_1 _ _ subset_preorder PSCL (composes PScompose) _ _ (magicwand_r PScompose)); auto.
+    + rewrite map_app; auto.
+  - rewrite <- (app_nil_l (map _ _)) ; apply list_compose_monot_cons with (□ (PMval atN) ⟜ □ (Int A)).
+    + eapply (@magicwand_r_eq_1 _ _ subset_preorder PSCL (composes PScompose) _ _ (magicwand_r PScompose)); auto.
+    + rewrite <- (app_nil_r _); rewrite <- ? app_assoc.
+      apply sem_rimp_l, sem_monad_l, (@sem_monad_r _ PMPS); list_simpl; auto.
+      apply (m_pwr_neutrality_r (@PS_neutral_r _ PMPS)).
+  - simpl; rewrite app_assoc; apply list_compose_monot_cons with (□ (Int A) ⊸ □ (Int B)); list_simpl; auto.
+    eapply (@magicwand_l_eq_1 _ _ subset_preorder PSCL (composes PScompose) _ _ (magicwand_l PScompose)); auto.
+  - apply list_compose_monot_cons with (□ (Int A) ⊸ □ (PMval atN)); list_simpl.
+    + eapply (@magicwand_l_eq_1 _ _ subset_preorder PSCL (composes PScompose) _ _ (magicwand_l PScompose)); auto.
+    + rewrite <- (app_nil_l _); apply sem_limp_l, sem_monad_l; auto.
+      apply sem_monad_r, (m_pwr_neutrality_r (@PS_neutral_r _ PMPS)).
+  - etransitivity; [ apply IHpi | apply cl_monotone ]; intros z Hz; simpl; auto.
+  - etransitivity; [ apply IHpi | apply cl_monotone ]; intros z Hz; simpl; auto.
+  - apply sem_cut with (□ (Int A)); auto.
+  - apply PMgax.
+  Unshelve. all: try apply PScl_stable_l; try apply PScl_stable_r.
+  Qed.
+
+End PhaseSpaces.
+
